spec/Wots.ec
@@ -17,11 +17,15 @@ clone import Subtype as LEN_N with
    proof *.
 
 
-type wots_message = nbytes.
+type wots_message = nbytes. (* TODO: CONFIRMAR *)
 type pkey = len_n_bytes.
 type skey = len_n_bytes.
 type wots_keypair = pkey * skey.
 type wots_signature = len_n_bytes.
+
+op from_int_list (x : int list) : byte list = map W8.of_int x.
+
+(* Imperative definition of WOTS+ *)
 
 module WOTS = {
   proc genSK() : skey = {
@@ -45,6 +49,7 @@ module WOTS = {
     var pk_i, sk_i : nbytes;
 
     while (i < len) {
+      address <- set_chain_addr address i;
       sk_i <- nth witness sk i;
       pk_i <- chain sk_i 0 (w - 1) _seed address;
       pk <- put pk i pk_i;
@@ -64,20 +69,93 @@ module WOTS = {
     return (pk, sk);
   }
 
-  proc sign(M : wots_message, sk : skey, _seed : seed, address : adrs) : wots_signature = {
-    var  csum : W32.t;
+  proc sign(m : wots_message, sk : skey, _seed : seed, address : adrs) : wots_signature = {
+    var csum : W8.t <- W8.zero;
+    var m_i : W8.t;
+    var sig : wots_signature;
+    var sig_i : nbytes;
+    var sk_i : nbytes;
+    var msg_i : int;
+    var _m : int list;
+    var i : int <- 0;
+    var len_2_bytes : W8.t;
 
-    var tmp_pk : wots_signature;
+    sig <- witness; (* To remove warning [warning] [Wots.ec:164] these procedures may use uninitialized local variables: - Top.WOTS.sign -> [sig] *)
 
-    (* TODO: *)
 
-    return tmp_pk;
+    (* Convert message to base w *)
+    _m <@ BaseW.base_w(m, len1);
+    m <- from_int_list _m;
+
+    (* Compute checksum *)
+    while (i < len1) {
+      m_i <- nth witness m i;
+      csum <- csum + W8.of_int(w - 1) - m_i;
+      i <- i + 1;
+    }
+
+    (* Convert checksum to base w *)
+    csum <- csum `<<` W8.of_int (8 - ((ceil (len2%r * log2(w%r))) %% 8));
+    len_2_bytes <- W8.of_int (ceil ((ceil (len2%r * log2(w%r)))%r / 8%r));
+
+    (* FIXME: TODO: *)
+    (* msg = msg || base_w(toByte(csum, len_2_bytes), w, len_2); *)
+
+    i <- 0;
+    while (i < len) {
+      address <- set_chain_addr address i;
+      sk_i <- nth witness sk i;
+      msg_i <- W8.to_uint (nth witness m i);
+      sig_i <- chain sk_i 0 msg_i _seed address;
+      sig <- put sig i sig_i;
+      i <- i + 1;
+    }
+
+    return sig;
   }
 
-  proc pkFromSig(M : wots_message, sig : wots_signature, _seed : seed, address : adrs) : pkey = {
+  proc pkFromSig(m : wots_message, sig : wots_signature, _seed : seed, address : adrs) : pkey = {
     var tmp_pk : pkey;
-    
-(* TODO *)
+    var csum : W8.t <- W8.zero;
+    var pk_i : nbytes;
+    var m_i : W8.t;
+    var _m : int list;
+    var i : int <- 0;
+    var len_2_bytes : W8.t;
+    var sig_i : nbytes;
+    var msg_i : int;
+
+    (* To remove this warning: [warning] [Wots.ec:166] these procedures may use uninitialized local variables:
+     - Top.WOTS.pkFromSig -> [tmp_pk] *)
+    tmp_pk <- witness;
+
+    (* Convert message to base w *)
+    _m <@ BaseW.base_w(m, len1);
+    m <- from_int_list _m;
+
+    (* Compute checksum *)
+    while (i < len1) {
+      m_i <- nth witness m i;
+      csum <- csum + W8.of_int(w - 1) - m_i;
+      i <- i + 1;
+    }
+
+    (* Convert checksum to base w *)
+    csum <- csum `<<` W8.of_int (8 - ((ceil (len2%r * log2(w%r))) %% 8));
+    len_2_bytes <- W8.of_int (ceil ((ceil (len2%r * log2(w%r)))%r / 8%r));
+
+    (* FIXME: TODO: *)
+    (* msg = msg || base_w(toByte(csum, len_2_bytes), w, len_2); *)
+
+    i <- 0;
+    while (i < len) {
+      address <- set_chain_addr address i;
+      sig_i <- nth witness sig i;
+      msg_i <- W8.to_uint (nth witness m i);
+      pk_i <- chain sig_i msg_i (w - 1 - msg_i) _seed address;
+      tmp_pk <- put tmp_pk i pk_i; 
+      i <- i + 1;
+    }
 
     return tmp_pk;
   }
@@ -89,6 +167,9 @@ module WOTS = {
   }
 
 }.
+
+(* Functional definition of WOTS+ *)
+
 op sample_n_bytes : nbytes -> nbytes.
 op genSKWots (sk : skey) = map sample_n_bytes sk.
 
@@ -99,6 +180,7 @@ op map1 ['a] (f : nbytes -> nbytes) (xs : (nbytes * 'a) list) =
 
 op genPKWots (pk : pkey, sk : skey, _seed : seed, address : adrs) : pkey =
   let keypair = zip pk sk in
+  (* FIXME: Address needs to be updated here *)
   let f : nbytes -> nbytes = fun sk_i => chain sk_i 0 (w-1) _seed address in
   unzip1 (map1 f keypair).
 
